rocq/theories/product.v
@@ -35,7 +35,17 @@ Section Product.
     Definition right_proj :
         list ((label1 * label2) * (node1 * node2)) -> list (label2 * node2) :=
             map (fun x => (snd (fst x), snd (snd x))).
+
+    Lemma fst_fst_left_proj :forall p,  map fst (map fst p) = map fst (left_proj p).
+    Proof.
+        induction p; cbn; [reflexivity| now rewrite IHp].
+    Qed.        
     
+    Lemma snd_fst_right_proj : forall p,  map snd (map fst p) = map fst (right_proj p).
+    Proof.
+        induction p; cbn; [reflexivity| now rewrite IHp].
+    Qed.  
+
 
     Lemma path_left_proj : 
         forall n p, path product n p ->
@@ -97,25 +107,125 @@ Section Product.
             apply H_path_product.
     Qed.
 
-    Section valid_proj.
+    Section valid_lang.
 
-        Variable Σ2 Σ3 : Type.
+        Variable Σ1 Σ2 Σ3 : Type.
         Variable sat_product : (label1 * label2) -> Σ3 -> Prop.
-        Variable sat : label2 -> Σ2 -> Prop.
-        Variable transf : Σ3 -> Σ2.
-        Variable H : forall a b, sat_product a b -> sat (snd a) (transf b).
+        Variable sat1 : label1 -> Σ1 -> Prop.
+        Variable transf1 : Σ3 -> Σ1.
+        Variable H1 : forall a b, sat_product a b -> sat1 (fst a) (transf1 b).
 
-        Lemma valid_right_proj : 
+
+        Lemma valid_left_proj : 
             forall tr p, valid sat_product p tr -> 
-                valid sat (List.map snd p) (List.map transf tr).
+                valid sat1 (List.map fst p) (List.map transf1 tr).
         Proof.
             induction tr as [|a tr IHtr]; 
                 intros [|p] H_valid; inversion H_valid as [|? ? ? ? Hvsp Hsp]; subst; simpl.
             -   constructor. 
-            -   apply IHtr in Hvsp. specialize (H _ _ Hsp). constructor ; assumption.
+            -   apply IHtr in Hvsp. specialize (H1 _ _ Hsp). constructor ; assumption.
         Qed.
 
-    End valid_proj.
+        Variable sat2 : label2 -> Σ2 -> Prop.
+        Variable transf2 : Σ3 -> Σ2.
+        Variable H2 : forall a b, sat_product a b -> sat2 (snd a) (transf2 b).
+
+        Lemma valid_right_proj : 
+            forall tr p, valid sat_product p tr -> 
+                valid sat2 (List.map snd p) (List.map transf2 tr).
+        Proof.
+            induction tr as [|a tr IHtr]; 
+                intros [|p] H_valid; inversion H_valid as [|? ? ? ? Hvsp Hsp]; subst; simpl.
+            -   constructor. 
+            -   apply IHtr in Hvsp. specialize (H2 _ _ Hsp). constructor ; assumption.
+        Qed.
+
+        Lemma language_left_proj : forall p w, language_wit sat_product product p w ->  
+            language_wit sat1 atm1 (left_proj p) (List.map transf1 w).
+        Proof.
+            intros. inversion H. constructor.
+            - now apply path_left_proj in H0.
+            - apply valid_left_proj in H3. now rewrite <- fst_fst_left_proj. 
+        Qed.
+
+        Lemma language_right_proj : forall p w, language_wit sat_product product p w ->  
+            language_wit sat2 atm2 (right_proj p) (List.map transf2 w).
+        Proof.
+            intros. inversion H. constructor.
+            - now apply path_right_proj in H0.
+            - apply valid_right_proj in H3.  now rewrite <- snd_fst_right_proj. 
+        Qed.
+
+    End valid_lang.
+
+
+    Section Properties.
+        Variable Σ1 Σ2 Σ3 : Type.
+        Variable sat_product : (label1 * label2) -> Σ3 -> Prop.
+        Variable sat1 : label1 -> Σ1 -> Prop.
+        Variable transf1 : Σ3 -> Σ1.
+        Variable H1 : forall a b, sat_product a b -> sat1 (fst a) (transf1 b).
+        Variable sat2 : label2 -> Σ2 -> Prop.
+        Variable transf2 : Σ3 -> Σ2.
+        Variable H2 : forall a b, sat_product a b -> sat2 (snd a) (transf2 b).
+
+
+        Lemma prod_complete : 
+            aut_complete _ _ atm1 -> 
+            aut_complete _ _ atm2 ->
+            aut_complete _ _ product.
+        Proof.
+            intros * Ha Hb n H.
+            assert (Hr1: reachable atm1 (fst n)).
+            {
+                destruct n.
+                simpl.
+                apply reachable_left_proj in H.
+                apply H.
+            }
+            assert (Hr2: reachable atm2 (snd n)).
+            {
+                destruct n.
+                apply reachable_right_proj in H.  
+                apply H.
+            }
+            apply Ha in Hr1 as [f [n1 Hat]].
+            apply Hb in Hr2 as [g [m1 Hbt]].
+            exists (f,g), (n1,m1).
+            split; assumption.
+        Qed.
+
+
+        Lemma prod_deterministic : 
+            aut_deterministic _ _ _ sat1 atm1 ->
+            aut_deterministic _ _ _ sat2 atm2 ->
+            aut_deterministic _ _ _ sat_product product.
+        Proof.
+            intros Ha Hg. red. split.
+            - intros [l l'] m [l1 l1'] m' s [Ht1 Hs1] [Ht2 Hs2]. destruct Ht1, Ht2.
+            destruct Ha as [Ha _], Hg as [Hg _].
+            apply H1 in Hs1 as Hs1a. apply H2 in Hs1 as Hs1g.
+            apply H1 in Hs2 as Hs2a. apply H2 in Hs2 as Hs2g.
+
+            pose proof (Ha _ _ _ _ _ (conj H Hs1a) (conj H3 Hs2a)).
+            pose proof (Hg _ _ _ _ _ (conj H0 Hs1g) (conj H4 Hs2g)).
+            destruct H5, H6. destruct m, m'. cbn in *. now subst.
+
+            - intros s w. destruct w. 
+                + intros. inversion H. inversion H5.
+                + intros [[p1 p2] [p3 p4]] p [n1 n1'] [n2 n2'] [l1 l1'] [l2 l2'] Hw [Ht1 Ht2] [Ht'1]. 
+                    apply language_left_proj with (transf1:=transf1) (sat1:=sat1) in Hw as Hw_left; [|assumption].
+                    apply language_right_proj with (transf2:=transf2) (sat2:=sat2) in Hw as Hw_right; [|assumption].
+                    destruct Ht1, Ht'1.
+                    destruct Ha as [_ Ha], Hg as [_ Hg]. cbn in *.
+                    apply H1 in Ht2 as Ht1. apply H2 in Ht2.
+                    apply H1 in H as H'. apply H2 in H.
+
+                    epose proof Ha _ _ _ _ _ _ _ _ Hw_left (conj H0 Ht1) (conj H4 H'). 
+                    epose proof Hg _ _ _ _ _ _ _ _ Hw_right (conj H3 Ht2) (conj H5 H). destruct H6. destruct H7. now subst.
+        Qed.
+
+    End Properties.
 End Product.
 
 Arguments product [node1 node2 label1 label2].
